***NO_CI*** Working on the heap-memory style

examples/seplogic/Shallow.fst
@@ -1,45 +1,45 @@
 module Shallow
 
-open SepLogic.Heap
+open SepLogic.HeapMemory
 
 (* postcondition, a predicate on the return value and the output heap *)
-let post (a:Type) = a * heap -> Type0
+let post (a:Type) = a * memory -> Type0
 
 (* precondition, a predicate on the input heap *)
-let pre = heap -> Type0
+let pre = memory -> Type0
 
 (* wp *)
 let st_wp (a:Type) = post a -> pre
 
 (* result type parametrized by a post *)
-let result (a:Type) (post:post a) = x:(a * heap){post x}
+let result (a:Type) (post:post a) = x:(a * heap){post (fst x, heap_memory (snd x))}
 
 (* st computation, also parametrized by a post *)
-let st (a:Type) (wp:st_wp a) = post:post a -> h0:heap{wp post h0} -> GTot (squash (result a post))
+let st (a:Type) (wp:st_wp a) = 
+  post:post a -> h0:heap{wp post (heap_memory h0)} -> GTot (squash (result a post))
 
 (* return *)
 let return (#a:Type) (x:a)
-  : st a (fun post h0 -> emp h0 /\ post (x, h0))
+  : st a (fun post m0 -> m0 == emp /\ post (x, m0))
   = fun post h0 -> FStar.Squash.return_squash (x, h0)
 
-(* frame wp by partitioning h into h0 and h1, and then prove post on the resulting heap and h1 *)
-let frame_wp0 (#a:Type) (wp:st_wp a) (post:heap -> (a * heap) -> Type0) (h h0 h1:heap) =
-  disjoint_heaps h0 h1 /\ h == join_tot h0 h1 /\ wp (post h1) h0
+(* frame wp by partitioning a heap whose memory is m into h0 and h1, and then prove post on the resulting heap and h1 *)
+let frame_wp0 (#a:Type) (wp:st_wp a) (post:memory -> (a * memory) -> Type0) (m:memory) (h0 h1:heap) =
+  let m0 = heap_memory h0 in
+  let m1 = heap_memory h1 in 
+  disjoint_memories m0 m1 /\ m == (m0 <*> m1) /\ wp (post m1) m0
 
-(* frame_wp1 and frame_wp2 existentially quantify over h0 and h1 *)
-let frame_wp1 (#a:Type) (wp:st_wp a) (post:heap -> (a * heap) -> Type0) (h h0:heap) =
-  exists (h1:heap). frame_wp0 wp post h h0 h1
+let frame_wp1 (#a:Type) (wp:st_wp a) (post:memory -> (a * memory) -> Type0) (m:memory) (h0:heap) =
+  exists (h1:heap). frame_wp0 wp post m h0 h1
 
-let frame_wp (#a:Type) (wp:st_wp a) (post:heap -> (a * heap) -> Type0) (h:heap) =
-  (* expanded out:
-   * exists (h0:heap) (h1:heap). disjoint h0 h1 /\ h == join_tot h0 h1 /\ wp (post h1) h0
-   *)
-  exists (h0:heap). frame_wp1 wp post h h0
+let frame_wp (#a:Type) (wp:st_wp a) (post:memory -> (a * memory) -> Type0) (m:memory) =
+  exists (h0:heap). frame_wp1 wp post m h0
 
 (* the idea is to call frame_wp with (frame_post p)? yes, see frame below *)
-let frame_post (#a:Type) (p:post a) (h:heap) ((x, h1):(a * heap)) = p (x, join_tot h h1)
+let frame_post (#a:Type) (p:post a) (m0:memory) ((x, m1):(a * memory)) = disjoint_memories m0 m1 /\ p (x, m0 <*> m1)
 
 module S = FStar.Squash
+
 let bind_exists
   (#a:Type)
   (#b:Type)
@@ -52,42 +52,55 @@ let bind_exists
 val frame: #a:Type -> #wp:st_wp a -> f:st a wp
          -> st a (fun post -> frame_wp wp (frame_post post))
 //Expanded out:
-//         st a (fun post h -> exists h0 h1. disjoint h0 h1 /\ h == join_tot h0 h1 /\ wp (fun h0' -> post (x, (join_tot h0' h1))) h0
-let frame #a #wp f =
+//         st a (fun post m -> exists m0 m1. disjoint m0 m1 /\ m == m0 <*> m1 /\ wp (fun m0' -> disjoint m0' m1 /\ post (x, (join_tot m0' m1))) m0
+let frame #a #wp f = 
   fun post h ->
-    assert (frame_wp wp (frame_post post) h);  //from the refinement annotation on st type
-    let s = FStar.Squash.join_squash (FStar.Squash.get_proof (frame_wp wp (frame_post post) h)) in
-    bind_exists #(result a post) #heap #(frame_wp1 wp (frame_post post) h) s (fun h0 s' ->
-      assert (frame_wp1 wp (frame_post post) h h0);
-      bind_exists #(result a post) #heap #(frame_wp0 wp (frame_post post) h h0) s' (fun h1 _ ->
-        assert (frame_wp0 wp (frame_post post) h h0 h1);
-        //so now, h0 and h1 are the frames
-        let sqres : squash (result a (frame_post post h1)) = f (frame_post post h1) h0 in
-        S.bind_squash #(result a (frame_post post h1))
+    assert (frame_wp wp (frame_post post) (heap_memory h));
+    let s = FStar.Squash.join_squash (FStar.Squash.get_proof (frame_wp wp (frame_post post) (heap_memory h))) in
+    bind_exists #(result a post) #heap #(frame_wp1 wp (frame_post post) (heap_memory h)) s (fun h0 s' -> 
+      assert (frame_wp1 wp (frame_post post) (heap_memory h) h0);
+      bind_exists #(result a post) #heap #(frame_wp0 wp (frame_post post) (heap_memory h) h0) s' (fun h1 _ -> 
+        assert (frame_wp0 wp (frame_post post) (heap_memory h) h0 h1);
+        let sqres : squash (result a (frame_post post (heap_memory h1))) = f (frame_post post (heap_memory h1)) h0 in 
+        S.bind_squash #(result a (frame_post post (heap_memory h1)))
                       #(result a post)
-                      sqres (fun (x_h0':result a (frame_post post h1)) ->
-          let x, h0' = x_h0' in
-          let res = x, join_tot h1 h0' in  //AR: had to change the order of h1 and h0', joint_tot commutativity lemma?
-          FStar.Squash.return_squash res)))
+                      sqres
+                      (fun (x_h0':result a (frame_post post (heap_memory h1))) -> 
+                         let (x, h0') = x_h0' in
+                         let res = (x, join_tot h1 h0') in 
+                         FStar.Squash.return_squash res)))
 
 val bind (#a:Type) (#wp1:st_wp a)
          (#b:Type) (#wp2:a -> st_wp b)
          (f:st a wp1)
          (g: (x:a -> st b (wp2 x)))
-    : st b (fun post h ->
-            frame_wp wp1 (frame_post (fun (x, h1) ->
-              frame_wp (wp2 x) (frame_post post) h1)) h)
+    : st b (fun post m ->
+            frame_wp wp1 (frame_post (fun (x, m1) ->
+              frame_wp (wp2 x) (frame_post post) m1)) m)
 let bind #a #wp1 #b #wp2 f g =
     fun post h ->
-      let sq_1 : squash (result a (fun (x, h1) -> frame_wp (wp2 x) (frame_post post) h1)) =
-        frame f (fun (x, h1) -> frame_wp (wp2 x) (frame_post post) h1) h in
-      S.bind_squash sq_1 (fun (x, h1) ->
-      frame (g x) post h1)
+      let sq_1 : squash (result a (fun (x, m1) -> frame_wp (wp2 x) (frame_post post) m1)) =
+        frame f (fun (x, m1) -> frame_wp (wp2 x) (frame_post post) m1) h in
+      S.bind_squash sq_1 (fun (x, m1) ->
+      frame (g x) post m1)
 
-let read (#a:Type) (r:ref a)
-  : st a (fun post h0 -> (exists (x:a). (r |> x) h0 /\ post (x, h0)))
-  = fun post h0 -> FStar.Squash.return_squash (sel_tot h0 r, h0)
+let alloc (#a:Type0) (x:a)
+  : st (ref a) (fun post m0 -> m0 == emp /\ (exists (r:ref a) . post (r, (r |> x))))
+  = fun post h0 ->
+      assert (heap_memory h0 == emp);
+      let (r,h1) = alloc h0 x in
+      assert (heap_memory h1 == (r |> x));
+      admit ()
+      //FStar.Squash.return_squash ()
 
-let write (#a:Type) (r:ref a) (v:a)
-  : st unit (fun post h0 -> (exists (x:a). (r |> x) h0 /\ (forall h1. (r |> v) h1 ==> post ((), h1))))
-    = fun post h0 -> FStar.Squash.return_squash ((), upd_tot h0 r v)
+let read (#a:Type0) (r:ref a)
+  : st a (fun post m0 -> (exists (x:a). m0 == (r |> x) /\ post (x, m0)))
+  = fun post h0 -> 
+      assert (mcontains (heap_memory h0) r);
+      FStar.Squash.return_squash (sel_tot h0 r, h0)
+
+let write (#a:Type0) (r:ref a) (v:a)
+  : st unit (fun post m0 -> (exists (x:a). m0 == (r |> x) /\ (forall m1. m1 == (r |> v) ==> post ((), m1))))
+    = fun post h0 -> 
+        assert (mcontains (heap_memory h0) r);
+        FStar.Squash.return_squash ((), upd_tot h0 r v)
